lean/Shars/Verification/Simple/SpongeAbsorb.lean
@@ -1,0 +1,1014 @@
+import Aeneas
+import Shars.BitVec
+import Shars.ArrayExtract
+import Shars.Definitions.Simple
+import Sha3.Spec
+import Aeneas.SimpLists.Init
+import Sha3.Facts
+import Init.Data.Vector.Lemmas
+import Init.Data.Nat.Basic
+import Init.Data.Array
+import Shars.Verification.Simple.Utils
+import Shars.Verification.Simple.Refinement
+import Shars.Verification.Simple.Auxiliary
+import Shars.Verification.Simple.KeccakP
+import Shars.Verification.Simple.ListIR
+
+set_option maxHeartbeats 100000
+attribute [-simp] List.getElem!_eq_getElem?_getD
+attribute [ext (iff := false)] List.ext_getElem!
+/- attribute [simp] Aeneas.Std.Slice.set -/
+
+#check Nat.div_le_div_right
+
+example(a b c: Nat): 0 < b → a * b < c → a ≤ c / b := by
+  intros b_pos a_b_lt_c
+  calc a
+    _ = (a * b) / b := by
+      rw [Nat.mul_div_cancel (H:=b_pos)]
+    _ ≤ c / b := by
+      apply Nat.div_le_div_right
+      simp [*, le_of_lt]
+
+-- attribute [simp_lists_simps] List.length_append List.take_append_eq_append_take List.take_zipWith List.length_zipWith List.length_take List.take_all_of_le List.length_drop List.drop_eq_nil_of_le List.drop_append_eq_append_drop List.nil_append List.zipWith_nil_left List.append_nil List.drop_drop List.take_take
+
+theorem getElem!_padding(x m: Nat)(i: Nat)
+: (Spec.«pad10*1» x m)[i]! = if i = 0 ∨ i = (Spec.«pad10*1» x m).size - 1 then true else false
+:= by
+  split
+  case isTrue h =>
+    simp [Spec.«pad10*1»]
+    obtain h | h := h
+    · simp [h]; congr
+    · simp [h, Spec.«pad10*1»]; congr
+  case isFalse h =>
+    by_cases i_idx: i < (Spec.«pad10*1» x m).size
+    case neg => simp [getElem!_neg, i_idx]
+    simp [Spec.«pad10*1»] at h i_idx ⊢
+    simp_ifs
+    rw [getElem!_pos]
+    case h => scalar_tac
+    simp
+
+theorem ref.mod_manipulation(a b r: Nat)
+  (h1: r ≥ 6)
+  (h2: a < r)
+  (h3: b <= 4)
+  (h4: (a + b) ≥ r)
+: ((- (a + b + 2: Int)) % r).toNat = 2*r - (a + b + 2)
+:= by
+  have: ((- (a + b + 2: Int)) % r) ≡ 2*r - (a + b + 2) [ZMOD r] := by
+    ring_nf
+    calc _
+      _ ≡ -2 + (-a.cast + -b.cast) [ZMOD r] := by apply Int.mod_modEq
+      _ ≡ -2 + (-a.cast + -b.cast) + r [ZMOD r] := by exact Int.ModEq.symm Int.add_modEq_right
+      _ ≡ -2 + (-a.cast + -b.cast) + r + r [ZMOD r] := by exact Int.ModEq.symm Int.add_modEq_right
+      _ ≡ -2 + (-a.cast + -b.cast) + 2* r [ZMOD r] := by ring_nf; rfl
+    ring_nf; rfl
+  have := this.eq
+  simp [Int.emod_emod] at this ⊢
+  simp [this]
+  have: (2*r - (a + b + 2): Int) >= 0 := by omega
+  have: (2*r - (a + b + 2): Int) < r := by omega
+  rw [Int.emod_eq_of_lt]
+  case H1 => omega
+  case H2 => omega
+  zify
+  rw [Int.toNat_of_nonneg (by omega)]
+  rw [Nat.cast_sub (by omega)]
+  simp
+
+open Aeneas hiding Std.Array
+open Std.alloc.vec
+
+theorem Spec.«pad10*1_length» (x m : Nat)
+: (Spec.«pad10*1» x m).size = (2 + (-(m + 2: Int) % x).toNat)
+:= by
+  simp_arith [«pad10*1», neg_add, -neg_add_rev, -Int.reduceNeg]
+  rfl
+
+def spec_sponge (r: Nat)(r_pos: r > 0):=
+  have: NeZero r := ⟨Nat.not_eq_zero_of_lt r_pos⟩
+  Spec.sponge (f := Spec.Keccak.P 6 24) (pad := Spec.«pad10*1»)
+def spec_sponge_absorb (r: Nat)(r_pos: r > 0) :=
+  have: NeZero r := ⟨Nat.not_eq_zero_of_lt r_pos⟩
+  Spec.sponge.absorb (f := Spec.Keccak.P 6 24) (pad := Spec.«pad10*1») (r := r)
+def spec_sponge_squeze{m d}(r: Nat)(r_pos: r > 0) :=
+  have: NeZero r := ⟨Nat.not_eq_zero_of_lt r_pos⟩
+  Spec.sponge.squeeze (m := m) (d := d) (f := Spec.Keccak.P 6 24) (r := r)
+
+/- #check BitVec.setWidth_cast -/
+
+def absorb.upd(S: BitVec (Spec.b 6))(P: Vector Bool r): BitVec (Spec.b 6) :=
+  Spec.Keccak.P 6 24 (S ^^^ (BitVec.ofBoolListLE <| P.toList).setWidth (Spec.b 6))
+
+def absorb{r: Nat}(S: BitVec (Spec.b 6))(Ps: Array (Vector Bool r)) := Id.run do
+  let mut S := S
+  for P in Ps do
+    S := absorb.upd S P
+  return S
+
+def simple.sponge_absorb_final.panic_free
+  (keccak_p: List Bool → List Bool)
+  (r: Nat)
+  (s rest suffix: List Bool)
+: List Bool
+:= Id.run do
+  let mut s := s
+  s := ListIR.xor_long s rest
+  let nb_left := rest.length + suffix.length
+  if nb_left >= r then
+    s := ListIR.xor_long_at s (suffix.take (r - rest.length)) rest.length
+  -- if nb_left >= r then
+    s := keccak_p s
+    s := ListIR.xor_long s (suffix.drop (r - rest.length))
+    s := ListIR.xor_long_at s [true] (rest.length + suffix.length - r)
+    s := ListIR.xor_long_at s [true] (r-1)
+  else
+    s := ListIR.xor_long_at s suffix rest.length
+    s := ListIR.xor_long_at s [true] nb_left
+    if nb_left + 1 < r then
+      s := ListIR.xor_long_at s [true] (r-1)
+    else
+      s := keccak_p s
+      s := ListIR.xor_long_at s [true] (r-1)
+  keccak_p s
+
+
+@[scalar_tac_simps]
+theorem Nat.sub_div_self(a b: Nat)
+:(a - b) / b = a / b - 1 := by
+  by_cases b > 0
+  case neg h => simp at h; subst h; simp
+  by_cases a >= b
+  case pos h =>
+    have: a = (a - b) + b := (Nat.sub_eq_iff_eq_add h).mp rfl
+    rw [this, Nat.add_sub_cancel, Nat.add_div_right, Nat.add_sub_cancel]
+    assumption
+  case neg h =>
+    simp at h
+    simp [Nat.div_eq_of_lt h, Nat.sub_eq_zero_of_le (le_of_lt h)]
+
+@[scalar_tac_simps]
+theorem Nat.sub_div_mult_left(a b: Nat)
+:(a - b*i) / b = a / b - i := by
+  by_cases b > 0
+  case neg h => simp at h; subst h; simp
+  case pos =>
+    cases i
+    case zero => simp
+    case succ i' =>
+      simp [Nat.mul_add, Nat.sub_add_eq, Nat.sub_div_self]
+      rw [Nat.sub_div_mult_left]
+
+theorem BitVec.cast_xor(bv bv2: BitVec n)(eq: n = m)
+: (bv ^^^ bv2).cast eq = bv.cast eq ^^^ bv2.cast eq
+:= by ext i i_lt; simp
+
+attribute [simp] Aeneas.Std.core.slice.index.Slice.index
+
+@[simp]
+-- theorem Array.toList_chunks_exact(arr: Array α)(k: Nat)
+-- : (arr.chunks_exact k).toList = (arr.toList.chunks_exact k).attach.map (fun data => ⟨data.val.toArray, by
+--     have := data.property
+--     simp [List.mem_iff_get] at this
+--     obtain ⟨_ , len⟩ := this
+--     simp [getElem_eq_getElem!, ←len]
+--     rw [List.length_getElem!_chunks_exact]
+--     omega
+--   ⟩)
+-- := by
+--   rw [chunks_exact]
+--   split
+--   case isTrue h =>
+--     simp
+--     rw [List.chunks_exact]
+--     simp [h]
+--   case isFalse h =>
+--     simp only [not_or] at h
+--     simp [Array.toList_chunks_exact]
+--     conv => rhs; arg 2;
+--     have: arr.toList.chunks_exact k = _ := rfl
+--     conv at this => rhs; rw [List.chunks_exact]; simp [*]
+--     rw [this]
+--     have : arr = arr.take k ++ arr.drop k := by exact?
+--     sorry
+
+private theorem List.foldl_congr{ls ls': List α}
+: ls = ls'
+→ upd = upd'
+→ init = init'
+→ ls.foldl upd init = ls'.foldl upd' init'
+:= by rintro rfl rfl rfl; rfl
+
+set_option maxRecDepth 1000000 in
+set_option maxHeartbeats 1000000 in
+theorem absorb.refinement{r: Nat}(S: BitVec (Spec.b 6))(bs: Array Bool)
+: (absorb S (bs.chunks_exact r)).toList = ListIR.absorb' ListIR.list_keccak_p S.toList (bs.toList.chunks_exact r)
+:= by
+  unfold absorb ListIR.absorb'
+  simp [ListIR.list_keccak_p, ListIR.xor_long.def, -Array.size_chunks_exact]
+  rw [←Array.foldl_toList]
+  rw [Array.chunks_exact, List.chunks_exact]
+  split <;> simp_ifs
+  case isTrue h =>
+    simp
+    ext i
+    · simp [Spec.b, Spec.w]
+    by_cases i < 1600 <;> simp
+    case pos h => intros; assumption
+    case neg h =>
+      rw [getElem!_neg]
+      case h => simpa using h
+      simp
+  case isFalse h =>
+    simp
+    generalize_proofs _ len_extract
+    have ih := @absorb.refinement r (@upd r S ⟨bs.extract 0 r, len_extract⟩) (bs.extract r)
+    simp [absorb,ListIR.absorb', ListIR.list_keccak_p, ListIR.xor_long.def] at ih
+    rw [ih]
+    rw [List.foldl_congr]
+    · simp_lists
+    · ext s chunk
+      · simp
+      simp
+    · rw [upd]
+      simp [List.setWidth, Spec.b, Spec.w]
+      rw [List.take_of_length_le (by simp)]
+      apply congrArg
+      apply congrArg
+      ext i i_idx
+      rw [ListIR.xor_long, ListIR.xor_long_at]
+      simp at i_idx
+      simp [←Bool.default_bool,←List.getElem!_eq_getElem?_getD, i_idx]
+      simp_lists
+      simp [i_idx]
+      split
+      · rename_i i_le_r
+        simp_lists [getElem_eq_getElem!]
+      · rename_i i_gt_r
+        simp_lists
+        simp [getElem_eq_getElem!]
+        congr
+        omega
+termination_by bs.size
+
+abbrev ref.interesting_part_of_the_proof.preconditions(r: Nat)(s rest suffix: List Bool) :=
+  r ≥ 6 -- Otherwise, we don't have suffix + 2 ≤ r
+∧ suffix.length ≤ 4 -- Taken from the actual uses of `suffix` in SHA3
+∧   rest.length < r -- Since rest is what's left after absorb_initial
+∧ s.length = 1600 -- The state has length Spec.b 6
+
+set_option maxRecDepth 100000000 in
+set_option maxHeartbeats 1000000 in
+theorem ref.interesting_part_of_the_proof.case1{r: Nat}{s rest suffix: List Bool}
+  (hyp: (rest ++ suffix).length ≥ r)
+: preconditions r s rest suffix
+→ let padding := (Spec.«pad10*1» r (rest.length + suffix.length)).toList
+  (rest ++ suffix ++ padding).chunks_exact r = [(rest ++ suffix).take r, (suffix.drop (r - rest.length) ++ padding)]
+:= by
+  /-
+  · (rest ++ suffix) >= r
+    Then we have
+     (rest ++ suffix ++ padding).chunks_exact k =
+     = [(rest ++ suffix).take r, (suffix.drop (r - rest.length) ++ padding)]
+  -/
+  rintro ⟨r_big_enough,suffix_len_le,rest_len_lt,len_s⟩ padding
+  have len_padding: (Spec.«pad10*1» r (rest.length + suffix.length)).size = 2*r - (rest.length + suffix.length) := by
+    simp [Spec.«pad10*1_length», -neg_add_rev]
+    have := mod_manipulation (h1 := r_big_enough) (h2 := rest_len_lt) (h3 := suffix_len_le) (h4 := by scalar_tac)
+    rw [this]
+    scalar_tac
+  have len_append: (rest.length + suffix.length + padding.length) = 2*r := by
+    simp [padding, len_padding]
+    scalar_tac
+  simp at hyp
+  have len_chunks: ((rest ++ suffix ++ padding).chunks_exact r).length = 2 := by
+    simp
+    rw [←Nat.add_assoc, len_append, Nat.mul_div_cancel]
+    omega
+
+  -- Execute List.chunks_exact
+  unfold List.chunks_exact
+  simp_ifs
+  unfold List.chunks_exact
+  simp_ifs
+  unfold List.chunks_exact
+  simp_ifs
+
+  congr 1
+  · ext i
+    · simp [←Nat.add_assoc, len_append]
+      omega
+    by_cases i < r
+    case neg => simp_lists
+    rw [List.getElem!_take_append_beg]
+    case pos.x => assumption
+    case pos.x => simp; omega
+    rw [List.getElem!_take]
+    case pos.a => assumption
+  · congr
+    ext i
+    · simp [←Nat.add_assoc, len_append]
+      omega
+    simp_lists
+    congr
+    omega
+
+set_option maxRecDepth 100000000 in
+set_option maxHeartbeats 1000000 in
+theorem ref.interesting_part_of_the_proof.case2{r: Nat}{s rest suffix: List Bool}
+  (hyp: (rest ++ suffix).length = r-1)
+: preconditions r s rest suffix
+→ let padding := (Spec.«pad10*1» r (rest.length + suffix.length)).toList
+  (rest ++ suffix ++ padding).chunks_exact r = [rest ++ suffix ++ [true], List.replicate (r-1) false ++ [true]]
+:= by
+  /-
+  · (rest ++ suffix) = r - 1
+    Then we have
+     (rest ++ suffix ++ padding).chunks_exact k =
+     = [rest ++ suffix ++ [true], List.replicate false (r-1) ++ [true]]
+  -/
+  rintro ⟨r_big_enough,suffix_len_le,rest_len_lt,len_s⟩ padding
+  have len_padding: (Spec.«pad10*1» r (rest.length + suffix.length)).size = 2*r - (rest.length + suffix.length) := by
+    simp at hyp
+    simp [Spec.«pad10*1_length», -neg_add_rev, hyp, r_big_enough]
+    zify
+    rw [Nat.cast_sub (by omega)]
+    rw [Nat.cast_sub (by omega)]
+    rw [Nat.cast_sub (by omega)]
+    rw [Nat.cast_mul]
+    ring_nf
+    simp
+    rw [
+      Int.neg_emod,
+      Int.emod_eq_of_lt (H1:=by omega) (H2:=by omega),
+      Int.max_eq_left (by omega)
+    ]
+    omega
+  have len_append: (rest.length + suffix.length + padding.length) = 2*r := by
+    simp [padding, len_padding]; scalar_tac
+
+  simp at hyp
+  have len_chunks: ((rest ++ suffix ++ padding).chunks_exact r).length = 2 := by
+    simp
+    rw [←Nat.add_assoc, len_append, Nat.mul_div_cancel]
+    omega
+
+  -- Execute List.chunks_exact
+  unfold List.chunks_exact
+  simp_ifs
+  unfold List.chunks_exact
+  simp_ifs
+  unfold List.chunks_exact
+  simp_ifs
+  congr
+  · ext i
+    · simp; scalar_tac
+    simp_lists
+    congr
+    simp [hyp, Nat.sub_sub_self, ‹r >= 1›', List.take_one, List.head?, padding, Spec.«pad10*1», BitVec.toList]
+  · ext i
+    · simp; scalar_tac
+    simp_lists
+    simp [hyp] at len_padding
+    simp [hyp, Nat.sub_sub_self, ‹r >= 1›', padding, Array.getElem!_toList, getElem!_padding, len_padding,
+       -Bool.if_false_right, -Bool.if_false_left, -Bool.if_true_left] -- Keep `if`s for `simp_ifs` to process
+    by_cases i = r -1
+    case pos h => simp_ifs [h]; simp
+    case neg =>
+      simp_ifs
+      by_cases i > r - 1
+      case neg => simp_ifs
+      case pos =>
+        simp_ifs
+        rw [getElem!_neg]
+        simp
+        scalar_tac
+
+set_option maxRecDepth 100000000 in
+set_option maxHeartbeats 1000000 in
+theorem ref.interesting_part_of_the_proof.case3{r: Nat}{s rest suffix: List Bool}
+  (hyp: (rest ++ suffix).length <= r-2)
+: preconditions r s rest suffix
+→ let padding := (Spec.«pad10*1» r (rest.length + suffix.length)).toList
+  (rest ++ suffix ++ padding).chunks_exact r = [rest ++ suffix ++ [true] ++ List.replicate (r -2 - rest.length - suffix.length) false ++ [true]]
+:= by
+  /-
+  · (rest ++ suffix) <= r - 2
+    Then we have
+     (rest ++ suffix ++ padding).chunks_exact k =
+     = [rest ++ suffix ++ [true, true]]
+  -/
+  rintro ⟨r_big_enough,suffix_len_le,rest_len_lt,len_s⟩ padding
+  have len_padding: (Spec.«pad10*1» r (rest.length + suffix.length)).size = r - (rest.length + suffix.length) := by
+    simp at hyp
+    simp [Spec.«pad10*1_length», -neg_add_rev]
+    zify
+    rw [Nat.cast_sub (by omega)]
+    rw [Int.neg_emod]
+    rw [Int.emod_eq_of_lt (H1:=by omega) (H2:=by omega)]
+    simp
+    rw [Int.max_eq_left (by omega)]
+    omega
+  have len_append: (rest.length + suffix.length + padding.length) = r := by
+    simp [padding, len_padding]
+    scalar_tac
+  have len_chunks: ((rest ++ suffix ++ padding).chunks_exact r).length = 1 := by
+    simp [←Nat.add_assoc, len_append, Nat.div_self, ‹r > 0›']
+
+  unfold List.chunks_exact
+  simp_ifs
+
+  unfold List.chunks_exact
+  simp_ifs
+  simp
+  ext i
+  · simp; scalar_tac
+  simp_lists
+  congr
+  simp [padding, Spec.«pad10*1», BitVec.toList]
+  have := Spec.«pad10*1_length» r (rest.length + suffix.length)
+  simp at this
+  ring_nf at this ⊢
+  scalar_tac
+
+set_option maxHeartbeats 1000000 in
+theorem ref.interesting_part_of_the_proof.proof(r: Nat)(s rest suffix: List Bool)
+: preconditions r s rest suffix
+→ let f := ListIR.list_keccak_p
+  let padding := (Spec.«pad10*1» r (rest.length + suffix.length)).toList
+  simple.sponge_absorb_final.panic_free f r s rest suffix =
+    ListIR.absorb' f s (
+      (rest ++ suffix ++ padding).chunks_exact r
+    )
+:= by
+  rintro precond f padding
+  have ⟨r_big_enough,suffix_len_le,rest_len_lt,len_s⟩ := precond
+  /-
+  There are three cases we must consider:
+  · (rest ++ suffix) >= r
+    Then we have
+     (rest ++ suffix ++ padding).chunks_exact k =
+     = [(rest ++ suffix).take r, (suffix.drop (r - rest.length) ++ padding)]
+  · (rest ++ suffix) = r - 1
+    Then we have
+     (rest ++ suffix ++ padding).chunks_exact k =
+     = [rest ++ suffix ++ [true], List.replicate false (r-1) ++ [true]]
+  · (rest ++ suffix) <= r - 2
+    Then we have
+     (rest ++ suffix ++ padding).chunks_exact k =
+     = [rest ++ suffix ++ [true, true]]
+  -/
+  if      cond1: (rest ++ suffix).length ≥ r then
+    rw [case1 cond1 precond]
+    simp at cond1
+    simp [ListIR.absorb', simple.sponge_absorb_final.panic_free, *, ListIR.xor_long]
+
+    generalize leftover_val: (rest.length + suffix.length - r) = leftover
+    rw [ListIR.xor_long_at_twice_separate]
+    case compatible_offset => scalar_tac
+
+    rw [ListIR.xor_long_at_twice_separate]
+    case compatible_offset => scalar_tac
+
+    rw [ListIR.xor_long_at_twice_separate]
+    case compatible_offset => scalar_tac
+
+    congr
+    · simp_arith [List.take_append_of_ge_length, le_of_lt rest_len_lt]
+    · simp_arith
+      scalar_tac
+    · have padding_len
+      : (Spec.«pad10*1» r (rest.length + suffix.length)).size = 2 * r - rest.length - suffix.length
+      := by
+        simp [Spec.«pad10*1»]
+        have: (2: Int) = (2: Nat).cast := by congr
+        rw [this]
+        have(a b: Int): a - b = a + -b := by exact rfl
+        rw [this]
+        simp only [←Nat.cast_sub, ←neg_add, Nat.cast_add]
+        conv =>
+          lhs
+          rhs
+          rw [Nat.cast_ofNat]
+          conv => enter [1, 1, 1, 1, 1]; rw [Int.add_comm]
+          rw [mod_manipulation (h1 := r_big_enough) (h2 := rest_len_lt) (h3 := suffix_len_le) (h4 := cond1)]
+        scalar_tac
+
+      ext i
+      · simp [padding_len]
+        scalar_tac
+      conv => rhs; rw [Array.getElem!_toList]
+      simp [getElem!_padding, -List.cons_append, -List.singleton_append, -List.cons_append_fun]
+      by_cases h: i = 0
+      case pos => simp [h]
+      by_cases h: i = (Spec.«pad10*1» r (rest.length + suffix.length)).size - 1
+      -- by_cases h: i = 2* r - rest.length - suffix.length - 1
+      case pos =>
+        rw [List.getElem!_append_right]
+        case h => scalar_tac
+        rw [List.getElem!_append_right]
+        case h => scalar_tac
+        simp [h, padding_len, ←leftover_val]
+        rw [List.getElem!_singleton]
+        scalar_tac
+      by_cases h: i < (Spec.«pad10*1» r (rest.length + suffix.length)).size
+      case neg =>
+        rw [getElem!_neg]
+        case h => simp [Spec.«pad10*1»] at *; scalar_tac
+        simp [Spec.«pad10*1»] at *
+        simp [*]
+      case pos =>
+        rw [getElem!_pos]
+        case h => simp [padding_len] at *; scalar_tac
+        rw [List.getElem_append_right]
+        case h₁ => scalar_tac
+        rw [List.getElem_append_left]
+        case h => scalar_tac
+        simp [padding_len] at *; simp [*]
+        scalar_tac
+
+  else if cond2: (rest ++ suffix).length = r - 1 then
+    rw [case2 cond2 precond]
+    replace cond2 := ‹r = (rest ++ suffix).length + 1›'
+    simp [ListIR.absorb', simple.sponge_absorb_final.panic_free, *, ListIR.xor_long]
+
+    rw [ListIR.xor_long_at_twice_separate]
+    case compatible_offset => scalar_tac
+
+    rw [ListIR.xor_long_at_twice_separate]
+    case compatible_offset => scalar_tac
+
+    simp [ListIR.xor_long_of_xor_long_at]
+    congr
+    -- have{α: Type}(x ls: List α): (x ++ ls) = ls ↔ x = [] := by exact?
+    simp_lists
+    scalar_tac
+
+  else if cond3: (rest ++ suffix).length ≤ r - 2 then
+    rw [case3 cond3 precond]
+    simp at cond3
+    simp [ListIR.absorb', simple.sponge_absorb_final.panic_free, *, ListIR.xor_long]
+    simp_ifs
+
+    rw [ListIR.xor_long_at_twice_separate]
+    case compatible_offset => scalar_tac
+
+    rw [ListIR.xor_long_at_twice_separate]
+    case compatible_offset => scalar_tac
+
+    rw [ListIR.xor_long_at_twice_separate]
+    case compatible_offset => scalar_tac
+
+    simp only [ListIR.xor_long_of_xor_long_at]
+    congr
+    · simp
+    · rw [List.append_right_eq_self, List.replicate_eq_nil_iff]
+      -- scalar_tac -- TODO: Gives maxRecDepth error
+      omega
+    · simp only [List.length_singleton, Nat.sub_add_eq]
+      congr
+
+  else omega -- Absurd
+
+theorem absorb_def{r: Nat}(S: BitVec (Spec.b 6))(Ps: Array (Vector Bool r))
+: absorb S Ps = Ps.foldl (absorb.upd · ·) S
+:= by simp [absorb]
+
+theorem absorb.spec (N : Array Spec.Bit) (r: Nat)(r_pos: r > 0)
+: spec_sponge_absorb r r_pos N = absorb (0#(Spec.b 6)) ((N ++ Spec.«pad10*1» r N.size).chunks_exact r)
+:= by
+  rw [spec_sponge_absorb, Spec.sponge.absorb, absorb]
+  -- NOTE: I needed to exercise a bit too much control here.
+  simp [←Array.foldl_toList,-Array.size_chunks_exact, -Array.size_map, upd]
+
+@[progress]
+theorem Aeneas.Std.Array.to_slice_mut.spec{α : Type u} {n : Usize} (a : Array α n)
+: ∃ old new,
+  Std.toResult (a.to_slice_mut) = .ok (old, new) ∧
+  old = a.to_slice ∧
+  new = a.from_slice
+:= by simp [to_slice_mut, Std.toResult]
+
+attribute [simp] Std.Slice
+set_option maxHeartbeats 1000000 in
+@[progress]
+theorem simple.sponge_absorb_initial_loop.spec
+  (bs : Std.Slice Bool) (r : Std.Usize) (s : Aeneas.Std.Array Bool 1600#usize) (n i : Std.Usize)
+: n.val = bs.length / r.val
+→ (r_pos: r.val > 0)
+→ i.val ≤ n.val
+→ r.val < 1600
+→ ∃ output,
+  sponge_absorb_initial_loop bs r s n i = .ok output ∧
+  output.val.toBitVec = (
+    (
+      absorb (s.val.toBitVec.cast (by simp [Spec.w, Spec.b])) (bs.val.toArray.chunks_exact r |>.drop i)
+    ).cast (by simp [Spec.w, Spec.b])
+  )
+:= by
+  rintro n_val r_pos i_idx r_le
+  rw [sponge_absorb_initial_loop]
+  split
+  case isTrue i_idx =>
+     -- r * i < r * n = r * (bs.length / r) ≤ bs.length ≤ Usize.max
+    have _: r.val*i.val ≤ bs.length := le_of_lt $ calc r.val * i.val
+        _ < r.val * n := Nat.mul_lt_mul_of_pos_left i_idx r_pos
+        _ = r.val * (bs.length / r) := by simp [n_val]
+        _ ≤ bs.length := Nat.mul_div_le bs.length ↑r
+
+     -- r * (i + 1) ≤ r * n = r * (bs.length / r) ≤ bs.length ≤ Usize.max
+    have _: r.val*(i.val + 1) ≤ bs.length := calc r.val * (i.val + 1)
+        _ ≤ r.val * n := Nat.mul_le_mul_left r.val i_idx
+        _ = r.val * (bs.length / r) := by simp [n_val]
+        _ ≤ bs.length := Nat.mul_div_le bs.length ↑r
+
+    let* ⟨ i1, i1_post ⟩ ← Std.Usize.mul_spec
+    let* ⟨ i2, i2_post ⟩ ← Std.Usize.add_spec
+    let* ⟨ i3, i3_post ⟩ ← Std.Usize.mul_spec
+    let* ⟨ slice, slice_post ⟩ ← Std.core.slice.index.Slice.index.slice_index_range_usize_slice_spec
+    fsimp only [*] at slice_post
+    let* ⟨old_slice, new_slice, slice_mut_post⟩ ← Std.Array.to_slice_mut.progress_spec
+
+    simp [Std.Array.to_slice_mut, Std.Array.to_slice] at slice_mut_post
+    obtain ⟨old_slice_post, new_slice_post⟩ := slice_mut_post
+
+    let* ⟨ s2, s2_len, s2_post ⟩ ← xor_long.spec
+    rw [old_slice_post] at s2_post
+    simp [s2_len] at s2_post
+
+    rw [slice_post] at s2_post
+    simp at s2_len
+    /- rw [s2_len] at s2_post -/ -- NOTE: Annoying that this doesn't work (setWidth's type depends on argument)
+
+    let* ⟨ s4, s4_post ⟩ ← keccak_p.spec
+    let* ⟨rest, rest_post ⟩ ← spec
+
+    simp [*]
+    apply congrArg
+    rw [absorb_def, absorb_def]
+    simp only [Array.foldl_extract]
+    rw [Array.foldl_step_right (l := i)]
+    case l_idx  | r_le | nontriv => (first | simp; done | simpa [n_val] using i_idx)
+    congr
+    ext idx idx_idx
+    simp [*]
+    rw [List.toBitVec] at s2_post
+    rw [←BitVec.getElem_ofBoolListLE, s2_post]
+    simp [Std.Array.from_slice, s2_post, old_slice_post, new_slice_post, ‹s2.length = 1600›']
+
+    rw [getElem_eq_getElem!,Array.getElem!_chunks_exact]
+    case i_idx | k_pos => (first | assumption | simpa [n_val] using i_idx)
+
+    simp
+  case isFalse i_oob =>
+    have := ‹bs.length / r.val - i.val = 0›'
+    simp [absorb, this, Array.foldl,Array.foldlM_start_stop (m := Id)]
+    rw [Array.extract_empty]
+    simp
+termination_by n.val - i.val
+decreasing_by scalar_decr_tac
+
+theorem Array.extract_start_stop(arr: Array α)
+(start_default : start = 0        := by omega)
+(stop_default :  stop  = arr.size := by omega)
+: arr.extract start stop = arr
+:= by subst start_default; subst stop_default; simp only [extract_size]
+
+@[progress]
+theorem simple.sponge_absorb_initial.spec
+  (bs : Std.Slice Bool) (r : Std.Usize) (s : Aeneas.Std.Array Bool 1600#usize)
+(r_pos: r.val > 0)
+: r.val < 1600
+→ s.val = List.replicate (Spec.b 6) false
+→ ∃ output,
+  sponge_absorb_initial bs r s = .ok output ∧
+  output.val = ListIR.absorb' ListIR.list_keccak_p s.val (bs.val.chunks_exact r)
+  -- ∧ output.val.toBitVec = ((absorb (s.val.toBitVec.cast (by simp; decide)) ((Array.mk bs.val).chunks_exact r)).cast (by simp; decide))
+:= by
+  intro r_lt s_zero
+  rw [sponge_absorb_initial]
+  let* ⟨ n, n_post ⟩ ← Std.Usize.div_spec
+  let* ⟨ res, res_post ⟩ ← simple.sponge_absorb_initial_loop.spec
+  simp [*, Array.extract_eq_self_of_le]
+
+  replace res_post := congrArg (f := BitVec.toList) res_post
+  simp at res_post
+  rw [res_post]
+
+  rw [Array.extract_start_stop (stop_default := by simp [*])]
+  rw [absorb.refinement]
+  simp [ListIR.absorb', s_zero]
+
+@[progress]
+theorem Aeneas.Std.core.slice.index.Slice.index_range_from_usize_spec(T: Type)
+(slice: Slice T)
+(i: ops.range.RangeFrom Usize)
+: i.start ≤ slice.length
+→ ∃ output,
+  Slice.index (Std.core.slice.index.SliceIndexRangeFromUsizeSlice T) slice i = .ok output ∧
+  output.val = slice.val.extract (start := i.start.val)
+:= by
+  intro inbound
+  simp only [index, SliceIndexRangeFromUsizeSlice.index]
+  simp_ifs
+  simp [Slice.drop]
+
+@[simp]
+def Aeneas.Std.UScalar.saturating_sub' {ty : UScalarTy} (x y : UScalar ty) : UScalar ty :=
+  UScalar.mk <| BitVec.ofFin ⟨x.val - y.val, Nat.lt_of_le_of_lt (Nat.sub_le _ _) x.bv.toFin.isLt⟩
+
+@[simp]
+theorem Aeneas.Std.UScalar.saturating_sub_def(a b: Std.UScalar ty)
+: a.saturating_sub b = a.saturating_sub' b
+:= by
+  simp only [saturating_sub, BitVec.ofNat, Fin.ofNat', saturating_sub']
+  simp
+  rw [Nat.mod_eq_of_lt]
+  exact Nat.lt_of_le_of_lt (Nat.sub_le _ _) a.bv.toFin.isLt
+
+/- attribute [scalar_tac_simps] Std.Array.to_slice -/
+-- TODO: Me da el límite de recursión, no se por qué.
+
+theorem Aeneas.Std.core.num.Usize.saturating_sub.spec(a b: Std.Usize)
+: ∃ c, Std.toResult (saturating_sub a b) = .ok c ∧ c.val = a.val - b.val
+:= by
+  simp [saturating_sub, UScalar.saturating_sub', Std.toResult]
+  reduce
+  rfl
+
+theorem Aeneas.Std.Array.to_slice_mut.spec'.{u} {α : Type u} {n : Std.Usize} (a : Aeneas.Std.Array α n)
+: ∃ old new, Std.toResult a.to_slice_mut = Std.Result.ok (old, new) ∧
+  old.val = a.val ∧ ∀ s: Slice α, (new s).val = (a.from_slice s).val
+:= by
+  progress as ⟨old, new, old_post, new_post⟩
+  simp [*, Std.Array.to_slice]
+
+
+@[progress]
+theorem simple.keccak_p.spec'(input: Aeneas.Std.Array Bool 1600#usize)
+: ∃ output,
+  keccak_p input = .ok output ∧
+  output.val = ListIR.list_keccak_p input.val
+:= by
+  rw [keccak_p, keccak_p_aux]
+  progress as ⟨res, res_post⟩
+  simp [ListIR.list_keccak_p]
+  simp  [StateArray.toSpec] at res_post
+  -- conv at res_post => arg 2; rw [StateArray.toSpec]
+  rw [Spec.Keccak.P.loop.spec, BitVec.setWidth_eq_cast]
+  case h => simp [Spec.b, Spec.w]
+  simp [←res_post]
+
+@[progress] theorem Aeneas.Std.Usize.sub_spec' {x y : Aeneas.Std.Usize} (h : y.val ≤ x.val) :
+  ∃ z, x - y = Std.Result.ok z ∧ z.val = x.val - y.val := by
+  progress as ⟨z, post⟩
+  rw [post, Nat.add_sub_cancel]
+
+@[progress]
+theorem simple.xor_long_at.spec'(a b: Std.Slice Bool)(offset: Std.Usize)
+: b.length + offset.val ≤ Std.Usize.max
+→ ∃ c,
+  xor_long_at a b offset = .ok c ∧
+  c.val = ListIR.xor_long_at a.val b.val offset.val
+:= by
+  intro nooverflow
+  let* ⟨ res, res_len, res_post ⟩ ← spec
+  ext i
+  · simp [res_len]
+  assume i_idx: i < res.length
+  case otherwise => simp_lists
+  rw [res_post, ListIR.getElem!_xor_long_at]
+  case a => assumption
+  simp [res_len] at i_idx
+  simp [i_idx]
+
+@[progress]
+theorem simple.xor_long.spec'(a b: Std.Slice Bool)
+: ∃ c,
+  xor_long a b = .ok c ∧
+  c.val = ListIR.xor_long a.val b.val
+:= by
+  rw [xor_long]
+  let* ⟨ res, post ⟩ ← xor_long_at.spec'
+  rw [post, ListIR.xor_long]
+
+
+/- set_option pp.coercions false in -/
+set_option maxHeartbeats 1000000 in
+@[progress]
+theorem simple.sponge_absorb_final.spec
+  (rest suffix : Std.Slice Bool) (r : Std.Usize) (s : Aeneas.Std.Array Bool _)
+: r.val ≥ 6
+→ rest.length < r
+→ suffix.length ≤ 4
+→ rest.length + suffix.length < Std.Usize.max
+→ ∃ output,
+  sponge_absorb_final s rest suffix r = .ok output ∧
+  output.val = sponge_absorb_final.panic_free ListIR.list_keccak_p r.val s.val rest.val suffix.val
+:= by
+  intro r_big_enough rest_lt suffix_le no_overflow
+  rw [sponge_absorb_final]
+
+  let* ⟨ old_s, mk_s1, old_s_post, new_s_post ⟩ ← Std.Array.to_slice_mut.spec'
+  let* ⟨ x1, x1_val ⟩ ← xor_long.spec'
+  -- ←Nat.sub_sub_eq_min
+  let* ⟨ nb_left, nb_left_post ⟩ ← Std.Usize.add_spec
+  simp at nb_left_post
+  split
+  case isTrue nb_left_ge_r =>
+    simp [nb_left_post] at nb_left_ge_r
+    let* ⟨ old_s1, mk_s2, old_s1_post, mk_s2_post ⟩ ← Std.Array.to_slice_mut.spec'
+    let* ⟨ i3, i3_post ⟩ ← Std.Usize.sub_spec'
+    simp at i3_post
+    let* ⟨ suffix_low, suffix_low_post ⟩ ← Std.core.slice.index.Slice.index.slice_index_range_usize_slice_spec
+    let* ⟨ x2, x2_val ⟩ ← xor_long_at.spec'
+    · simp [*]; scalar_tac
+    let* ⟨ x3, x3_val ⟩ ← keccak_p.spec'
+    let* ⟨ old_s2, mk_s3, old_s2_post, mk_s3_post ⟩ ← Std.Array.to_slice_mut.spec'
+    let* ⟨ suffix_high, suffix_high_post ⟩ ← Std.core.slice.index.Slice.index_range_from_usize_spec
+    let* ⟨ x4, x4_val ⟩ ← xor_long.spec'
+    let* ⟨ old_s3, mk_s4, old_s3_post, mk_s4_post ⟩ ← Std.Array.to_slice_mut.spec'
+    let* ⟨ single_one, single_one_post ⟩ ← Std.Array.to_slice.progress_spec
+    simp only [Std.toResult, Std.Array.make, Std.Array.to_slice] at single_one_post
+    let* ⟨ i7, i7_post ⟩ ← Std.Usize.sub_spec'
+    let* ⟨ x5, x5_val ⟩ ← xor_long_at.spec'
+    let* ⟨ old_s4, mk_s5,  old_s4_post, mk_s5_post ⟩ ← Std.Array.to_slice_mut.spec'
+    let* ⟨ i8, i8_post ⟩ ← Std.Usize.sub_spec'
+    let* ⟨ x6, x6_val ⟩ ← xor_long_at.spec'
+    let* ⟨ res, res_post_2 ⟩ ← keccak_p.spec'
+
+    simp [*, panic_free, Std.Array.from_slice, ListIR.xor_long]
+    simp_ifs
+    congr
+    simp_lists
+  case isFalse nb_left_idx =>
+    simp [nb_left_post] at nb_left_idx
+    let* ⟨ old_s1, mk_s2, old_s1_post, mk_s2_post ⟩ ← Std.Array.to_slice_mut.spec'
+    let* ⟨ s5, s5_val ⟩ ← xor_long_at.spec'
+    let* ⟨ _x_1, _x_2, _x_post_1, _x_post_2 ⟩ ← Std.Array.to_slice_mut.spec'
+    let* ⟨ single_one, single_one_post ⟩ ← Std.Array.to_slice.progress_spec
+    simp only [Std.toResult, Std.Array.make, Std.Array.to_slice] at single_one_post
+    let* ⟨ s9, s9_val ⟩ ← xor_long_at.spec'
+    let* ⟨ i3, i3_post ⟩ ← Std.Usize.add_spec
+    split
+    case isTrue nb_left_has_space =>
+      let* ⟨ _x_1, _x_2, _x_post_1, _x_post_2 ⟩ ← Std.Array.to_slice_mut.spec'
+      let* ⟨ i8, i8_post ⟩ ← Std.Usize.sub_spec'
+      let* ⟨ s19, s19_val ⟩ ← xor_long_at.spec'
+      let* ⟨ res, res_val ⟩ ← keccak_p.spec'
+
+      simp [*, panic_free, Std.Array.from_slice, ListIR.xor_long]
+      simp_ifs
+    case isFalse nb_left_has_space =>
+      let* ⟨ s11, s11_val ⟩ ← keccak_p.spec'
+      let* ⟨ _x_1, _x_2, _x_post_1, _x_post_2 ⟩ ← Std.Array.to_slice_mut.spec'
+      let* ⟨ i8, i8_post ⟩ ← Std.Usize.sub_spec'
+      let* ⟨ s19, s19_val ⟩ ← xor_long_at.spec'
+      let* ⟨ res, res_val ⟩ ← keccak_p.spec'
+
+      simp [*, panic_free, Std.Array.from_slice, ListIR.xor_long]
+      simp_ifs
+
+theorem List.chunks_exact_truncate{α: Type}(bs: List α)(r: Nat)
+: (bs.take (r*(bs.length/r))).chunks_exact r = bs.chunks_exact r
+:= by
+  assume r_pos: r > 0
+  case otherwise => simp at r_pos; subst r_pos; simp [List.chunks_exact]
+  have r_neZero: NeZero r := NeZero.of_pos r_pos
+  cases bs using List.cases_extract r
+  case onSmall small =>
+    unfold List.chunks_exact
+    simp [*]
+  case onBig chunk rest len_chunk =>
+    unfold List.chunks_exact
+    simp [*, r_neZero.out]
+    have: r <= r*(rest.length / r + 1) := by ring_nf; simp
+    have: rest.length / r + 1 = (chunk ++ rest).length / r := by simp [len_chunk, Nat.add_div_left, r_pos]
+    simp_lists [len_chunk]
+    simp_arith
+    ring_nf
+    simp_arith
+    apply List.chunks_exact_truncate
+termination_by bs.length
+decreasing_by simp [*]
+
+@[simp]
+theorem List.chunks_exact_nil(r: Nat): ([]: List α).chunks_exact r = [] := by unfold List.chunks_exact; simp
+
+theorem List.chunks_exact_split{α: Type}(bs: List α)(r: Nat)(i: Nat)
+: (bs.take (r*i)).chunks_exact r ++ (bs.drop (r*i)).chunks_exact r = bs.chunks_exact r
+:= by
+  assume r_pos: r > 0
+  case otherwise => simp at r_pos; simp [r_pos]
+
+  ext j : 1
+  · simp
+    by_cases r*i ≥ bs.length
+    case pos h => simp [h]
+    case neg h =>
+      simp at h
+      have : i ≤ bs.length / r := by
+        simp only [Nat.le_div_iff_mul_le r_pos, h, le_of_lt, Nat.mul_comm i]
+      simp [h, le_of_lt, Nat.sub_div_mult_left, Nat.mul_div_cancel_left, r_pos, this]
+  assume h: r*i < bs.length
+  case otherwise =>
+    simp at h
+    rw [List.take_of_length_le h]
+    rw [List.drop_of_length_le h]
+    simp
+  have: i ≤ bs.length / r := by
+    simp only [Nat.le_div_iff_mul_le r_pos, h, le_of_lt, Nat.mul_comm i]
+  assume j < bs.length / r
+  case otherwise h =>
+    simp at h
+    rw [getElem!_neg]
+    rw [getElem!_neg]
+    · simp; omega
+    · simp [*, le_of_lt, Nat.sub_div_mult_left]
+
+  by_cases j < i
+  case pos j_lhs =>
+    rw [List.getElem!_append_left]
+    case h => simp [*, le_of_lt, Nat.mul_div_cancel, r_pos]
+    rw [List.getElem!_chunks_exact]
+    case a => simp [*, le_of_lt, Nat.mul_div_cancel, r_pos]
+    rw [List.getElem!_chunks_exact]
+    case a => simp; omega
+    simp
+    rw [List.take_drop]
+    rw [List.take_drop]
+    rw [List.take_take]
+    congr
+    ring_nf
+    simp
+    have : r*(j + 1) ≤ r*i := by
+      apply Nat.mul_le_mul_left
+      assumption
+    simpa [Nat.mul_add] using this
+  case neg j_rhs =>
+    simp at j_rhs
+    rw [List.getElem!_append_right]
+    case h => simp [*, le_of_lt]
+    rw [List.getElem!_chunks_exact]
+    case a => simp [*, le_of_lt, Nat.sub_div_mult_left]; omega
+    rw [List.getElem!_chunks_exact]
+    case a => simp [*]
+    simp [*, le_of_lt]
+    congr 1
+    · ring_nf; simp [Nat.mul_sub]
+    · congr
+      simp [Nat.mul_sub, *]
+
+
+/- @[progress] -/
+set_option maxRecDepth 1000000 in
+theorem simple.sponge_absorb.spec_list
+  (bs : Std.Slice Bool) (r : Std.Usize) [NeZero r.val](input : Aeneas.Std.Array Bool 1600#usize)
+  (suffix : Std.Slice Bool)
+: r.val ≥ 6
+→ r.val < 1600
+→ suffix.length ≤ 4
+→ input.val = List.replicate 1600 false
+→ let padding := (Spec.«pad10*1» r.val (bs.length % r.val + suffix.length)).toList
+∃ output,
+  sponge_absorb bs r input suffix = .ok output ∧
+  -- output.
+  -- output.val.toBitVec = (spec_sponge_absorb r.val (Nat.pos_of_neZero r.val) (bs.val.toArray ++ suffix.val.toArray)).cast (by simp [Spec.b, Spec.w])
+  -- absorb → absorb'
+  output.val =
+    ListIR.absorb' ListIR.list_keccak_p input.val (
+      (bs.val ++ suffix.val ++ padding).chunks_exact r
+    )
+:= by
+  intro r_big_enough r_bounded suffix_small input_zero
+  unfold sponge_absorb
+  have r_pos: r.val > 0 := by omega
+
+  let* ⟨ s1, s1_post ⟩ ← sponge_absorb_initial.spec
+  let* ⟨ n, n_post ⟩ ← Std.Usize.div_spec
+  have := Nat.mul_div_le bs.length r
+  let* ⟨ i1, i1_post ⟩ ← Std.Usize.mul_spec
+  let* ⟨ rest, rest_post ⟩ ← Std.core.slice.index.Slice.index_range_from_usize_spec
+  have rest_len: rest.length < r := by simp [*, ←Nat.mod_eq_sub, Nat.mod_lt]
+  let* ⟨ res, res_post ⟩ ← sponge_absorb_final.spec
+
+  simp only [*]
+  rw [ref.interesting_part_of_the_proof.proof]
+  case a =>
+    simp [ref.interesting_part_of_the_proof.preconditions, *, ←Nat.mod_eq_sub, Nat.mod_lt]
+  simp [-List.reduceReplicate, ←Nat.mod_eq_sub, Nat.mod_lt]
+  generalize (Spec.«pad10*1» r.val (bs.length % r.val + suffix.length)).toList = padding
+  rw [ListIR.absorb'_absorb']
+  congr
+  rw [List.take_of_length_le (h := by simp [Nat.add_comm (bs.length % r), Nat.div_add_mod])]
+
+  rw [←List.chunks_exact_truncate]
+
+  rw [←List.append_assoc]
+  rw [←List.drop_append_of_le_length (by scalar_tac)]
+  rw [←List.drop_append_of_le_length (by trans bs.length <;> (first | assumption | simp))]
+  rw [←List.take_append_of_le_length (l₂ := suffix.val) (by assumption)]
+  rw [←List.take_append_of_le_length (l₂ := padding) (by trans bs.length <;> (first | assumption | simp))]
+  rw [List.chunks_exact_split, List.append_assoc]
