lean/Shars/Verification/Simple/SpongeSqueeze.lean
@@ -1,0 +1,354 @@
+import Aeneas
+import Shars.BitVec
+import Shars.ArrayExtract
+import Shars.Definitions.Simple
+import Sha3.Spec
+import Aeneas.SimpLists.Init
+import Sha3.Facts
+import Init.Data.Vector.Lemmas
+import Init.Data.Nat.Basic
+import Init.Data.Array
+import Shars.Verification.Simple.Utils
+import Shars.Verification.Simple.Refinement
+import Shars.Verification.Simple.Auxiliary
+import Shars.Verification.Simple.KeccakP
+import Shars.Verification.Simple.ListIR
+
+set_option maxHeartbeats 100000
+attribute [-simp] List.getElem!_eq_getElem?_getD
+attribute [ext (iff:=false)] List.ext_getElem!
+
+-- attribute [scalar_tac_simps] Nat.pos_of_neZero
+
+@[scalar_tac inst]
+def Nat.pos_of_neZero'{n: Nat}(inst: NeZero n): n > 0 := @Nat.pos_of_neZero n inst
+
+#check simple.sponge_squeeze_loop
+
+def simple.sponge_squeeze.panic_free(r: Nat)[NeZero r](dst s: List Bool)(offset: Nat): List Bool :=
+  assert! s.length ≥ r
+  if offset + r < dst.length then
+    let dst' := dst.replace_slice offset (offset + r) (s.take r)
+    let s' := ListIR.list_keccak_p s
+    panic_free r dst' s' (offset + r)
+  else
+    let nb_left := dst.length - offset
+    dst.replace_slice offset (offset + nb_left) (s.take nb_left)
+termination_by dst.length - offset
+decreasing_by simp [List.replace_slice]; scalar_tac
+
+def simple.sponge.squeeze.length_panic_free(r: Nat)(dst s: List Bool)(offset: Nat)
+  (r_pos: r > 0)
+  (r_lt: r < 1600)
+: s.length ≥ r
+→ have: NeZero r := {out := Nat.not_eq_zero_of_lt r_pos}
+  (simple.sponge_squeeze.panic_free r dst s offset).length = dst.length
+:= by
+  intro s_big_enough
+  unfold simple.sponge_squeeze.panic_free
+  simp only [s_big_enough, reduceIte]
+  split
+  case isTrue h =>
+    rw [simple.sponge.squeeze.length_panic_free]
+    case r_pos => assumption
+    case r_lt => assumption
+    case a => simp; omega
+    simp [List.replace_slice, h, le_of_lt, s_big_enough, ←Nat.add_assoc, ‹offset ≤ dst.length›',]
+  case isFalse h =>
+    simp [List.replace_slice, h, le_of_lt, s_big_enough, ←Nat.add_assoc]
+    simp only [Nat.min_def]
+    simp_ifs
+    split <;> simp at * <;> simp [*, Nat.sub_eq_zero_of_le, le_of_lt]
+termination_by dst.length - offset
+decreasing_by simp [List.replace_slice]; scalar_tac
+
+attribute [scalar_tac_simps] not_le in
+def ListIR.sponge.squeeze(d: Nat)(r: Nat)[NeZero r](dst s: List Bool): List Bool :=
+  if d ≤ dst.length then
+    dst.take d
+  else
+    squeeze d r (dst ++ s.setWidth r) (ListIR.list_keccak_p s)
+termination_by d - dst.length
+decreasing_by scalar_decr_tac
+
+
+theorem List.getElem!_replace_slice[Inhabited α](ls ls2: List α)(s e: Nat)
+: s ≤ e -- Proper range
+→ e ≤ ls.length -- e goes up to end
+→ s < ls.length -- s goes up to last
+→ (ls.replace_slice s e ls2)[i]! =
+    if       i < s              then ls[i]!
+    else if  i - s < ls2.length then ls2[i - s]!
+    else ls[i - (s + ls2.length) + e]!
+:= by
+  intros
+  simp [replace_slice]
+  split_ifs <;> simp_lists
+  rw [Nat.add_comm, Nat.sub_add_eq]
+
+
+attribute [scalar_tac_simps] List.length_setWidth
+
+theorem List.getElem!_take_eq_ite[Inhabited α](ls: List α)(n i: Nat)
+: (ls.take n)[i]! = if i < n then ls[i]! else default
+:= by split <;> simp_lists
+
+
+attribute [simp_lists_simps] List.getElem!_take_eq_ite in
+theorem simple.sponge_squeeze.panic_free.spec(r: Nat)
+  (r_bnd: 0 < r ∧ r < 1600)
+  (dst s: List Bool)(offset : Nat)
+: s.length = 1600
+→ offset < dst.length
+→ have: NeZero r := {out := Nat.not_eq_zero_of_lt r_bnd.left}
+  panic_free r dst s offset = ListIR.sponge.squeeze dst.length r (dst.take offset) s
+:= by
+  intro len_s offset_idx
+  simp
+  unfold panic_free ListIR.sponge.squeeze
+  simp_ifs
+  split
+  case isTrue next_offset_lt =>
+    have: (List.replace_slice offset (offset + r) dst (List.take r s)).length = dst.length := by
+      simp [List.replace_slice]; scalar_tac
+    rw [spec r r_bnd]
+    case a => simp
+    case a => simp [*]
+    congr 1
+    ext i
+    · simp [*, le_of_lt]
+    assume i < offset + r
+    case otherwise => simp_lists
+    simp_lists [List.getElem!_replace_slice]
+  case isFalse next_offset_lt =>
+    unfold ListIR.sponge.squeeze
+    simp_ifs
+    ext i
+    · simp [*, List.replace_slice]; scalar_tac
+    simp_lists [List.getElem!_replace_slice]
+    simp_ifs
+termination_by dst.length - offset
+decreasing_by scalar_decr_tac
+
+
+
+
+
+
+
+
+
+
+
+
+
+
+
+
+
+
+
+
+
+
+
+
+
+
+
+abbrev List.is_chunks_of(chunks: List (List α))(n: Nat) := ∀ c ∈ chunks, c.length = n
+
+@[simp_lists_simps]
+theorem List.length_flatten_of_is_chunks(n: Nat)(chunks: List (List α))
+: chunks.is_chunks_of n
+→ chunks.flatten.length = chunks.length * n
+:= by
+  intro is_chunks
+
+  induction chunks
+  case nil => simp
+  case cons hd tl ih =>
+    simp [List.is_chunks_of] at *
+    obtain ⟨len_hd, len_flatten_tl⟩ := is_chunks
+    rw [ih (is_chunks := len_flatten_tl)]
+    simp_arith [*, Nat.add_mul]
+
+@[simp_lists_simps]
+theorem List.getElem!_cons_div_of_gt[Inhabited α](i n: Nat)(hd: α)(tl: List α)
+: n > 0 → i ≥ n → (hd :: tl)[i / n]! = tl[(i - n) / n]!
+:= by
+  intro n_pos h
+  have: i = (i - n) + n := by exact (Nat.sub_eq_iff_eq_add h).mp rfl
+  conv => lhs; rw [this, Nat.add_div_right (H := n_pos)]
+  simp
+
+@[simp_lists_simps]
+theorem List.getElem!_cons_div_of_lt[Inhabited α](i n: Nat)(hd: α)(tl: List α)
+: i < n → (hd :: tl)[i / n]! = hd
+:= by intro h; simp [Nat.div_eq_of_lt, h]
+
+@[simp_lists_simps]
+theorem List.getElem!_flatten_of_is_chunks(n: Nat)[Inhabited α](chunks: List (List α))
+: chunks.is_chunks_of n
+→ ∀ i, chunks.flatten[i]! = (chunks[i/n]!)[i%n]!
+:= by
+  intro is_chunks
+
+  assume n_pos: n > 0
+  case otherwise =>
+    simp at n_pos
+    intro i
+    rw [getElem!_default, getElem!_default]
+    · if inside: i / n < chunks.length then
+        rw [getElem!_pos]
+        case h => assumption
+        have := is_chunks (chunks[i / n]) (by simp)
+        simp [*]
+      else
+        rw [getElem!_neg]
+        case h => assumption
+        simp [default]
+    · rw [List.length_flatten_of_is_chunks (n:=n)]
+      · simp [*]
+      · assumption
+
+  induction chunks
+  case nil => simp [default]
+  case cons hd tl ih =>
+    intro i
+    simp [List.is_chunks_of] at *
+    obtain ⟨len_hd, len_flatten_tl⟩ := is_chunks
+    replace ih := ih len_flatten_tl
+    by_cases i < n
+    case pos i_hd =>
+      simp_lists
+      simp [Nat.div_eq_of_lt, Nat.mod_eq_of_lt,i_hd]
+    case neg i_tl =>
+      simp at i_tl
+      simp_lists
+      rw [ih]
+      simp [len_hd, Nat.mod_eq_sub_mod, i_tl]
+
+@[simp_lists_simps]
+private theorem List.getElem!_iterate[Inhabited α](f: α → α)(a: α)(n i: Nat)
+: (List.iterate f a n)[i]! = if i < n then f^[i] a else default
+:= by
+  split
+  case isTrue i_idx  => simp [getElem!_pos, i_idx]
+  case isFalse i_oob => simp [getElem!_neg, i_oob]
+
+-- def List.sumWhileNotGt(ls: List Nat)(top: Nat) := Id.run do
+--   let mut sum := 0
+--   for x in ls do
+--     if sum + x > top then
+--       break
+--     sum := sum + x
+--   return sum
+
+-- theorem List.getElem_flatten[Inhabited α](ls: List (List α))(i: Nat)
+-- : let n := ls.map (·.length) |>.sumWhileNotGt i
+--   ls.flatten[i]! = (ls[n]!)[i - n]!
+-- := by sorry
+
+def ref.squeeze(s: List Bool)(n: Nat)(k: Nat := 1600)[NeZero k] :=
+  (List.iterate list_keccak_p (s.setWidth k) n).flatten
+
+attribute [-simp] List.mem_iterate in
+@[simp, simp_lists_simps]
+theorem iterate_list_keccak_p_is_chunks_of_1600(s: List Bool)(n: Nat)
+: (List.iterate ref.list_keccak_p (s.setWidth 1600) n).is_chunks_of 1600
+:= by
+  induction n generalizing s
+  case zero => simp [List.is_chunks_of]
+  case succ d' ih =>
+    unfold List.is_chunks_of at *
+    simp
+    intros chunk chunk_prev
+    rw [ih (s := ref.list_keccak_p (s.setWidth 1600))]
+    simp [*]
+
+-- private theorem length_squeeze(n: Nat)(s: List Bool)
+-- : (ref.squeeze s n 1600).length = n*1600
+-- := by
+--   unfold ref.squeeze
+--   rw [List.length_flatten_of_is_chunks 1600]
+--   case a => apply iterate_list_keccak_p_is_chunks_of_1600
+--   simp [ref.squeeze]
+
+-- private theorem getElem!_squeeze(n: Nat)(s: List Bool)
+-- : (ref.squeeze s n 1600)[i]! = (ref.list_keccak_p^[i / 1600] s.setWidth)[i % 1600]!
+-- := by
+--   simp [ref.squeeze]
+--   ref [List.getElem!_flatten_of_is_chunks]
+--   sorry
+
+attribute [-simp] List.length_flatten in
+attribute [simp] length_iterate_keccak_p in
+set_option maxHeartbeats 100000000 in
+theorem simple.sponge_squeze_loop.spec (r i: Std.Usize)(input: Std.Slice Bool)(s: Aeneas.Std.Array Bool 1600#usize)
+: r.val < 1600
+→ i < input.length
+→ i.val % r.val = 0
+→ input.length + r.val < Std.Usize.max
+→ ∃ output,
+  sponge_squeeze_loop r input s i = .ok output ∧
+  output.length = input.length ∧
+  output.val = input.val.take i.val ++ ref.squeeze s.val ((input.length - i.val) / r)
+  /- output.val[j]! = input. -/
+  /- (∀ j < output.length, output.val[j]! = -/
+  /-   if i.val ≤ j then -/
+  /-     (ref.list_keccak_p s.val)[j]! -/
+  /-   else -/
+  /-     input.val[j]! -/
+:= by
+  intros r_lt i_idx i_mod_r no_overflow
+  unfold sponge_squeeze_loop
+  let* ⟨ s1, s1_def ⟩ ← Std.Array.to_slice.progress_spec
+  let* ⟨ nb_added, curr, nb_added_val, curr_len, curr_pt_val ⟩ ← add_to_vec.spec
+  · simp [*, Std.Array.to_slice]
+  let* ⟨ i1, i1_post ⟩ ← Std.Usize.add_spec
+  have: input.length ≤ (input.length / r) * 1600 := by sorry
+  split
+  case isTrue last_loop =>
+    simp [*]
+    ext j
+    · have this2: input.length - i ≤ input.length := by exact Nat.sub_le input.length i.val
+      simp [*, le_of_lt, _root_.trans this2 this]
+    assume j_idx: j < curr.length
+    case otherwise => simp_lists
+    rw [curr_pt_val]
+    case a => simpa [*] using j_idx
+    simp_lists
+    split
+    case isTrue cond =>
+      simp_ifs
+      rw [List.getElem!_flatten_of_is_chunks 1600]
+      case a => apply iterate_list_keccak_p_is_chunks_of_1600
+      simp_lists
+      have: j < (input.length / r) * 1600 := by
+        scalar_tac
+      sorry
+    rw [List.getElem!_flatten_of_is_chunks]
+    sorry
+  case isFalse has_more_loops =>
+    let* ⟨ s2, s2_post ⟩ ← keccak_p.spec'
+    let* ⟨ res, res_post_1, res_post_2 ⟩ ← spec
+
+    simp [*]
+
+theorem simple.sponge_squeze.spec (r: Std.Usize)(input: Std.Slice Bool)
+: ∃ output,
+  sponge_squeeze_loop r input s i = .ok output ∧
+  output.length = input.length ∧
+  output.val = (List.iterate ref.list_keccak_p s.val (input.length / r)).flatten.take (input.length - i.val)
+:= by
+  sorry
+
+-- @[progress]
+theorem simple.sponge.spec (r : Std.Usize) (bs output suffix: Std.Slice Bool)
+[NeZero r.val]
+/- (r_ne_zero: r.val ≠ 0) -/
+: ∃ output,
+  simple.sponge r bs output suffix = .ok output ∧
+  output.val = (Spec.sponge (f := Spec.Keccak.P 6 (nᵣ := 24)) (pad := Spec.«pad10*1») r.val (Array.mk <| bs.val ++ suffix.val ) output.length).toArray.toList
+:= by sorry
